---
cssclasses:
  - callouts-outlined
---
#### Hamilton's principle
A path that a particle follows that makes minimum action
$$S=\int_{p_1}^{p_2} dt\, L(x, \dot{x};t)$$ 
Given a stystem subject to a constant force, the equations of motion can be derived by applying Euler's equation to the functional $S$.
##### Free particle
Taking a Lagraingian that has the kintetic energy $T=0$, 
$$m\ddot{x}=\frac{d}{dt}\frac{\partial}{\partial\dot{x}}\left(\frac{1}{2}m\dot{x}^2\right)=0$$
$$S=\int_{p_1}^{p_2} dt\, \frac{1}{2}m\dot{x}^2$$
##### Free particle with force
$$F=m\ddot{x}\Rightarrow-\frac{\partial U}{\partial x}-m\ddot{x}=0$$
$$L=T-U=\frac{1}{2}m\dot{x}^2-U$$
>[!danger] Euler-Lagrange equation
>$$\frac{\partial \mathcal{L}(x,\dot{x};t)}{\partial x}-\frac{d}{dt}\left(\frac{\partial \mathcal{L}(x, \dot{x}; t)}{\partial \dot{x}}\right)=0$$

##### 3D Lagrangian
$$ \mathcal{L}=\mathcal{L}(x,y,z,\dot{x},\dot{y},\dot{z};t)=T-U$$
$$T=\frac{1}{2}m(\dot{x}^2+\dot{y}^2+\dot{z}^2)\hspace{10mm}U=U(x,y,z,t)$$
These equations can be solved individually for each coordinate to give $$m\ddot{x}=-\frac{\partial U}{\partial x}\hspace{7mm}m\ddot{y}=-\frac{\partial U}{\partial y}\hspace{7mm}m\ddot{z}=-\frac{\partial U}{\partial z}$$
#### Simple pendulum

![[Pasted image 20241120123657.png#invert_B | 200]]
>[!question] Solve with forces

Knowing that $\vec{F}=m\vec{a}$, $x$ is given by $$F_x=-mg\sin\theta=ma_x$$ and $y$ is given by $$F_y=-mg\cos\theta + T=ma_y=0$$
$$a_x=\frac{d}{dt}v_x = \frac{d}{dt}l\dot{\theta}=l\ddot{\theta}$$
This gives $$\ddot{\theta}+\frac{g}{l}\sin\theta=0$$
>[!question] Solve using Lagrangian

$$T=\frac{1}{2}mv^2=\frac{1}{2}ml^2\dot{\theta}^2\hspace{1cm} U=mgh=mg(l-l\cos\theta)=mgl(1-\cos\theta)$$
Solving for $\mathcal{L}(\theta, \dot{\theta};t)=T-U$, $$\frac{\partial\mathcal{L}}{\partial\theta}=mgl\sin\theta\hspace{1cm}\frac{\partial\mathcal{L}}{\partial\dot{\theta}}=\frac{1}{2}ml^2 2\dot{\theta}=ml^2 \dot{\theta}$$
Giving the same result as before after plugging into the Euler-Lagrange equation.
#### Double pendulum
Consider the following coordinate system, $$x_1=l_1\sin\theta_1\hspace{7mm}y_1=l_1\cos\theta_1\hspace{7mm}x_2=l_1\sin\theta_1+l_2\sin\theta_2\hspace{7mm}y_2=l_1\cos\theta_1-l_2\cos\theta_2$$
Constraining $x_1^2+y_1^2=l_1^2$ and $x_2^2+y_2^2=l_1^2+l_2^2+2l_1l_2\cos(\theta_1-\theta_2)\leq(l_1-l_2)^2$.
Writing the Lagrangian components, $$T=\frac{1}{2}m_x(\dot{x}_1^2+\dot{x}_2^2)+\frac{1}{2}m_y(\dot{y}_1^2+\dot{y}_2^2)\hspace{1cm} U=g(m_1y_1+m_2y_2)$$
Take the time derivative of the coordinates, the Lagrangian becomes $$\mathcal{L}=\left(\frac{m_1}{2}+\frac{m_2}{2}\right)l_1^2\dot{\theta}_1^2+\frac{m_2}{2}l_2^2\dot{\theta}_2^2+m_2l_1l_2\dot{\theta}_1\dot{\theta}_2\cos(\theta_1-\theta_2)+gl_1(m_1+m_2)\cos\theta_1+gm_2l_2\cos\theta_2$$
Then solving for $\mathcal{L}$ for the Euler-Lagrange equation, for $\theta_1$: $$\frac{\partial \mathcal{L}}{\partial \theta_1}=-m_2l_1l_2\dot{\theta}_1\dot{\theta}_2\sin(\theta_1-\theta_2)-gl_1(m_1+m_2)\sin\theta_1$$ $$\frac{\partial \mathcal{L}}{\partial \dot{\theta}_1}=\left(m_1+m_2\right)l_1^2\dot{\theta}_1+m_2l_1l_2\dot{\theta}_2\cos(\theta_1-\theta_2)$$
$$\frac{d}{dt}\frac{\partial \mathcal{L}}{\partial \dot{\theta}_1}=\left(m_1+m_2\right)l_1^2\ddot{\theta}_1+m_2l_1l_2\ddot{\theta}_2\cos(\theta_1-\theta_2)-m_2l_1l_2\dot{\theta}_2\sin(\theta_1-\theta_2)\dot{\theta}_1+m_2l_1l_2\dot{\theta}_2\sin(\theta_1-\theta_2)\dot{\theta}_2$$
And the same steps can be done for $\theta_2$. The final solution can be then be obtained using numerical analysis. 

>[!tip] Concervation laws
If $\mathcal{L}$ does not depend on $q_i$, the partial derivative of $\mathcal{L}$ with respect to $\dot{q}_1$ is constant, thus $q_i$ is a **conserved quantity**.

#### Particle on a cone
Take the following coordinates $$l\cos\alpha=z\hspace{7mm}l\sin\alpha=r\hspace{7mm}\frac{z}{r}=\cot\alpha$$
![[Pasted image 20241120123757.png#invert_B|400]]
And the standard $x\, y\, z$ transformation into the cyllindrical coordinates, $x = r\cos\theta$ and $y=r\sin\theta$

Getting the Lagrangian components, $$T=\frac{1}{2}m(\dot{r}^2+r^2\dot{\theta}^2+\dot{r}^2\cot^2\alpha) \hspace{1cm}U=mgr\cot\alpha$$
Giving the Lagrangian $\mathcal{L}=\mathcal{L}(r,\theta,\dot{r},\dot{\theta};t)$
Taking the Euler-Lagrange equations, $$\frac{d}{dt}\left(\frac{\partial \mathcal{L}}{\partial \dot{\theta}}\right)=0\hspace{1cm}\frac{\partial \mathcal{L}}{\partial \dot{\theta}}=mr^2\dot{\theta}$$
$$\frac{\partial \mathcal{L}}{\partial r}-\frac{d}{dt}\left(\frac{\partial \mathcal{L}}{\partial \dot{r}}\right)=0 \hspace{7mm} \frac{\partial \mathcal{L}}{\partial r} = mr\dot{\theta}^2-mg\cot\alpha \hspace{7mm} \frac{\partial \mathcal{L}}{\partial \dot{r}} = \frac{m\dot{r}}{\sin^2\alpha}$$
$$mr\dot{\theta}^2-mg\cot\alpha -\frac{m\ddot{r}}{\sin^2\alpha}=0$$
Knowing that $\dot{\theta}$ is constant and simplifying, 
$$\boxed{\ddot{r}-\frac{\sin^2\alpha}{r^3}C+\frac{g}{2}\sin2\alpha=0}
$$
![[cone.png#invert_B | 500]]

#### Holonomic constraints

Taking the sum, $$\sum^3A_i\dot{x}_i+B=\frac{df}{dt}=0$$ where $$A_i=\frac{\partial f}{\partial x_i}\hspace{1cm}B=\frac{\partial f}{\partial t}$$
>[!tip] Lagrange multipliers
>$$\frac{\partial \mathcal{L}}{\partial q_i}-\frac{d}{dt}\frac{\partial \mathcal{L}}{\partial \dot{q}_i}+\sum_{k=1}^m \lambda_k\frac{\partial f_k}{\partial q_i}=0$$
>Having the sum term defined as generalized force $Q_i$

#### Rolling disk
Taking $F(y, \theta)=0$, $F=y-R\theta$.

$$T = \frac{1}{2}m\dot{y}^2+\frac{1}{2}I\dot{\theta}^2=\frac{1}{2}m\dot{y}^2+\frac{1}{4}\dot{\theta}^2mR^2\hspace{1cm}U=mg(l-y)\sin\alpha$$

>[!question] 1 coordinate with minimal Euler-Lagrange equation

Taking $y=R\theta$, the Lagrangian becomes $$\mathcal{L} = \frac{1}{2}m\dot{y}^2+\frac{1}{4}\dot{\theta}^2mR^2+mg(R\theta-l)\sin\alpha$$
Solving the parts of the EL equation, $$\frac{\partial \mathcal{L}}{\partial \theta}=mgR\sin\alpha\hspace{1cm}\frac{\partial \mathcal{L}}{\partial \dot{\theta}}=\frac{3}{2}mR^2\dot{\theta}$$
Giving $$\ddot{\theta}=\frac{2}{3}\frac{g}{R}\sin\alpha$$
>[!question] 2 coordinates with minimal Euler-Lagrange equation with Lagrange multipliers

Keeping the full Lagrangian, $$\mathcal{L} = \frac{1}{2}m\dot{y}^2+\frac{1}{4}\dot{\theta}^2mR^2 + mg(y+l)\sin\alpha$$
Keeping $f=y-R\theta=0$,
$$\frac{\partial \mathcal{L}}{\partial y}-\frac{d}{dt}\left(\frac{\partial \mathcal{L}}{\partial \dot{y}}\right)+\lambda\frac{\partial f}{\partial y}=0 \hspace{1cm} \frac{\partial \mathcal{L}}{\partial \theta}-\frac{d}{dt}\left(\frac{\partial \mathcal{L}}{\partial \dot{\theta}}\right)+\lambda\frac{\partial f}{\partial \theta}=0$$
Giving $$\ddot{\theta}=\frac{2}{3}\frac{g}{R}\sin\alpha\hspace{7mm}\ddot{y}=\frac{2}{3}g\sin\alpha\hspace{7mm}\lambda=-\frac{1}{3}mg\sin\alpha$$
Thus generalized force is $Q_y = -(1/3)mg\sin\alpha$ and $Q_\theta=(1/3)mgR\sin\alpha$.
#### Equivalence of Lagrange and Newton approach
>[!question] Lagrange $\rightarrow$ Newton

Starting from $$\frac{\partial \mathcal{L}}{\partial x_i}-\frac{d}{dt}\frac{\partial\mathcal{L}}{\partial\dot{x}_i}=0$$ to arrive to $F_i=\dot{p}_i$
Plugging in $\mathcal{L} = T-U$, $$-\frac{\partial U}{\partial x_i}=\frac{d}{dt}\frac{\partial T}{\partial \dot{x}_i}$$
and for the conserved system $F_i$ is equal to the left hand side $$\frac{d}{dt}\frac{\partial T}{\partial \dot{x}_i}=\frac{d}{dt}\frac{\partial}{\partial \dot{x}_i}\sum_{j=1}^3\frac{1}{2}m\dot{x}_j^2=\frac{d}{dt}m\dot{x}_i=\dot{p}_i$$
>[!question] Newton $\rightarrow$ Lagrange

Transforming cartesian to generalized coordinates $x_i=x_i(q_j,t)$. The derivative of $x_i$ wrt $t$ is $$\dot{x}_i=\sum_j\frac{\partial x_i}{\partial q_j}\dot{q_j}+\frac{\partial x_i}{\partial t}$$
Generalized momentum is determined by $$p_j=\frac{\partial T}{\partial\dot{q}_j}=\sum_i\left(m\ddot{x}_i\frac{\partial x_i}{\partial q_j}+m\dot{x}_i\frac{d}{dt}\frac{\partial x_i}{\partial q_j\partial t}\right)$$ where $$\frac{d}{dt}\frac{\partial x_i}{\partial q_j\partial t}=\sum_k\frac{\partial^2 x_i}{\partial q_k\partial q_j}\dot{q}_j+\sum_i m\dot{x}_i\frac{\partial^2x_i}{\partial q_j\partial t}$$ giving $$\dot{p}_j=\sum_im\ddot{x}_i\frac{\partial x_i}{\partial q_j}+\sum_k\frac{\partial^2 x_i}{\partial q_k\partial q_j}\dot{q}_j+\sum_i m\dot{x}_i\frac{\partial^2x_i}{\partial q_j\partial t}$$
and the generalized force to be $$Q_j=\sum_iF_i\frac{\partial x_i}{\partial q_j}=-\frac{\partial U}{\partial q_j}$$
Defining $$\frac{\partial T}{\partial q_j}=\sum_im\dot{x}_i\frac{\partial \dot{x}_i}{\partial q_j}=\sum_im\dot{x}_i\frac{\partial }{\partial q_j}\left(\sum_j\frac{\partial x_i}{\partial q_j}\dot{q_j}+\frac{\partial x_i}{\partial t}\right)$$
so $\dot{p}_j=Q_j+\partial T/\partial q_j$, thus $$\frac{d}{dt}\frac{\partial T}{\partial \dot{q}_j}-\frac{\partial T}{\partial q_j}=-\frac{\partial U}{\partial q_j}$$
#### Noether's theorem
For each continuous symmetry of the Lagrangian there is a corresponding conserved quantity
##### Conservation of energy

>[!danger] Hamiltonian
>$$\mathcal{H}=\sum_j\dot{q}_j\frac{\partial\mathcal{L}}{\partial\dot{q}_j}-\mathcal{L}$$



Under some conditions, $\mathcal{H}=E=T+U$.
- $\partial U / \partial \dot{q}_j=0$, the potential energy does not depend on generalized velocities
- the transofrmation between the cartesian and generalized coordinates is independent of time, making the kitetic energy a homogenous quadratic function

#### Formulating equations of motion in terms of $\mathcal{H}$
$$\mathcal{H}(q_j,p_j;t)=\dot{q}_jp_j-\mathcal{L}(t, q_j, \dot{q}_j)$$
$$\frac{\partial\mathcal{H}}{\partial{q_j}}=-\dot{p}_j\hspace{1cm}\frac{\partial\mathcal{H}}{\partial{p_j}}=\dot{q}_j$$
Thus giving, $$\boxed{\frac{d\mathcal{H}}{dt}=-\frac{\partial\mathcal{L}}{\partial t}}$$
>[!tip] Generalized momentum
>$$p_j=\frac{\partial\mathcal{L}}{\partial\dot{q}_j}$$

>[!tip] Hamilton's equations
$$\frac{\partial\mathcal{H}}{\partial q_j}=-\dot{p}_j\hspace{1cm}\frac{\partial\mathcal{H}}{\partial p_j}=\dot{q}_j$$

Mass $m$ moving along $x$, $$F(x,t)=\frac{k}{x^2}e^{-t/\tau}$$
Finding $\mathcal{L}$, $$\frac{\partial U}{\partial x} = -F\hspace{3mm}\Rightarrow \hspace{3mm}U=-\int\frac{k}{x^2}e^{-t/\tau}\,dx=\frac{k}{x}e^{-t/\tau}$$
$$\mathcal{L}=\frac{1}{2}m\dot{x}-\frac{k}{x}e^{-t/\tau}$$
Finding $\mathcal{H}$, $$\mathcal{H}=\dot{x}\frac{\partial\mathcal{L}}{\partial\dot{x}}-\mathcal{L}=\frac{1}{2}m\dot{x}^2+\frac{k}{x}e^{-t/\tau}=T+U$$