#### Newton's Second Law in Non-Inertial Frames
Motion in inertial frame, $$\vec F = m\vec a$$
and in a non-inertial frame, $$\vec F' = m\vec a'$$
where $\vec F$ includes both real and fictitious forces
```tikz
\begin{document}
\begin{tikzpicture}[scale=.75]
%set text size to 14
\begin{scope}[font=\Large]

% axis xzy
\draw[->] (0,0) -- (5,0) node[right] {$x$};
\draw[->] (0,0) -- (0,5) node[above] {$z=z'$};
\draw[->] (0,0) -- (-2,-2) node[below] {$y$};
\draw[->] (0,0) -- (5, 3);

%put text at 6, 4
\node at (5.75,3.75) {$m$};
\node at (3,2.5) {$\vec r$};



%draw circle at 5,3
\draw[fill] (5,3) circle (0.2);


%axis x'y'z'
\draw[->, orange] (0,0) -- (5,1) node[right] {$x'$};

%red color line


\draw[->, orange] (0,0) -- (-1,-2) node[below] {$y'$};

\end{scope}
\end{tikzpicture}
\end{document}
```

Intetial frame rotating about $\hat z$ with angular velocity $\vec\omega=\omega\hat z$ 
$$\dot{\vec r} = \vec \omega \times \vec r$$
$$\dot{\hat e}_i' = \vec \omega \times \hat e_i', \hspace{7mm} i=1, 2, 3$$
In a non-inertial time, the velocity becomes, $$\dot{\vec r} = \dot{r'} \hat e_i' +  r' \dot{\hat e}_i' = \dot{r'} \hat e_i' +\vec \omega \times \vec r$$
The acceleration is then, $$\ddot{\vec r} = \ddot{r}_i' \hat e_i' + r_i'\vec\omega\times(\vec\omega\times\vec e_i') + 2\dot r_i'\vec\omega\times\vec e_i'+\dot{\vec\omega}\times\vec r $$
Obtaining the full equation,

>[!tip] Acceleration in a non-inertial frame
>$$ \left(\frac{d^2 \vec r}{dt^2}\right)_S = \left(\frac{d^2 \vec r}{dt^2}\right)_{S'} + \vec\omega\times(\vec\omega\times\vec r) + 2\vec\omega\times\left(\frac{d\vec r}{dt}\right)_{S'} + \frac{d\vec\omega}{dt}\times\vec r$$

Rewriting it in terms of forces, $$m\vec a' = \vec F - m \vec \omega \times (\vec \omega \times \vec r) - 2m\vec \omega \times \vec v' - m\dot{\vec \omega} \times \vec r$$
where, $\vec F$ is the real force and the other terms are fictitious forces. The fictitious forces are: 
$$\begin{align} \vec F_{\text{centrifugal}} &= -m\vec \omega \times (\vec \omega \times \vec r) \\
\vec F_{\text{Coriolis}} &= -2m\vec \omega \times \vec v' \\
\vec F_{\text{Euler}} &= -m\dot{\vec \omega} \times \vec r \end{align}$$
#### Earth as a non-inertial frame
The Euler force can be ignored as the Earth's axis completes a full circle over 26000 years

Taking the gravitational force to be $$\vec g_0 = -\frac{Gm}{r^2}\hat e_R$$ and being close to the surface $|\vec r| \ll |\vec R|$, $\dot{\vec R} = \vec\omega\times\vec R$ and $\ddot{\vec R} \approx \vec\omega\times(\vec\omega\times\vec R)$ , giving the total force, $$\vec F = m\vec g_0 - m\vec\omega\times(\vec\omega\times(\vec r +\vec R)) - 2m\vec\omega\times\vec v' - \vec \omega \times (\vec \omega \times \vec R)$$
and defining $\vec g = \vec g_0 - \vec\omega\times(\vec\omega\times\vec R)$, the total force becomes, $$\vec F = m\vec g - 2m\vec\omega\times\vec v'$$


